Add definitions to the Lean library

backends/lean/Aeneas/Std/Alloc.lean
@@ -10,7 +10,9 @@ open Result
 
 attribute [rust_type "alloc::string::String"] String
 
-/-- The type of the global allocator -/
+/-- The type of the global allocator - note it shouldn't appear in the generated code because
+    we systematically filter it when providing information about the definitions supported by the standard
+    libary. -/
 @[rust_type "alloc::alloc::Global"]
 inductive Global where | mk
 
@@ -19,6 +21,9 @@ def alloc.boxed.Box.deref {T : Type} (x : T) : T := x
 
 @[rust_fun "alloc::boxed::{core::ops::deref::DerefMut<Box<@T>, @T>}::deref_mut" -canFail (keepParams := [true, false])]
 def alloc.boxed.Box.deref_mut {T : Type} (x : T) : (T × (T → T)) := (x, λ x => x)
+
+@[rust_fun "alloc::alloc::{core::clone::Clone<alloc::alloc::Global>}::clone"]
+def alloc.alloc.CloneGlobal.clone (_ : Global) : Result Global := .ok .mk
 
 namespace Std
 
